refactor: modified each formatter to use the a default format that can be parsed by the date% macro

src/Std/Time/DateTime.lean
@@ -74,7 +74,17 @@ def toTimestampAssumingUTC (pdt : PlainDate) : Timestamp :=
 
 /--
 Calculates the duration between a given `PlainDate` and a specified date.
+
+## Example
+
+```lean
+def example : Duration :=
+  let startDate := date% 2023-1-1
+  let endDate := date% 2023-3-15
+  endDate.since startDate
+```
 -/
+@[inline]
 def since [ToTimestamp α] (date : PlainDate) (since : α) : Duration :=
   let date  := date.toTimestampAssumingUTC
   let since := ToTimestamp.toTimestamp since
@@ -122,7 +132,17 @@ instance : ToTimestamp PlainDate where
 
 /--
 Calculates the duration between a given `PlainDateTime` and a specified date.
+
+## Example
+
+```lean
+example : Duration :=
+  let startDate := date% 2023-1-1:05:10:20
+  let endDate := date% 2023-3-15:05:10:20
+  endDate.since startDate
+```
 -/
+@[inline]
 def since [ToTimestamp α] (date : PlainDateTime) (since : α) : Duration :=
   let date  := date.toTimestampAssumingUTC
   let since := ToTimestamp.toTimestamp since
