tests/lean/run/timeClassOperations.lean
@@ -18,49 +18,49 @@ info: 1970-01-08
 def datetime := date% 2000-01-20:03:02:01
 
 /--
-info: 2000-01-20 04:02:01.000000000
+info: 2000-01-20:04:02:01:000000000
 -/
 #guard_msgs in
 #eval datetime + (1 : Hour.Offset)
 
 /--
-info: 2000-01-20 02:02:01.000000000
+info: 2000-01-20:02:02:01:000000000
 -/
 #guard_msgs in
 #eval datetime - (1 : Hour.Offset)
 
 /--
-info: 2000-01-20 03:12:01.000000000
+info: 2000-01-20:03:12:01:000000000
 -/
 #guard_msgs in
 #eval datetime + (10 : Minute.Offset)
 
 /--
-info: 2000-01-20 02:52:01.000000000
+info: 2000-01-20:02:52:01:000000000
 -/
 #guard_msgs in
 #eval datetime - (10 : Minute.Offset)
 
 /--
-info: 2000-01-20 03:03:01.000000000
+info: 2000-01-20:03:03:01:000000000
 -/
 #guard_msgs in
 #eval datetime + (60 : Second.Offset)
 
 /--
-info: 2000-01-20 03:01:01.000000000
+info: 2000-01-20:03:01:01:000000000
 -/
 #guard_msgs in
 #eval datetime - (60 : Second.Offset)
 
 /--
-info: 2000-01-21 03:02:01.000000000
+info: 2000-01-21:03:02:01:000000000
 -/
 #guard_msgs in
 #eval datetime + (1 : Day.Offset)
 
 /--
-info: 2000-01-19 03:02:01.000000000
+info: 2000-01-19:03:02:01:000000000
 -/
 #guard_msgs in
 #eval datetime - (1 : Day.Offset)
@@ -68,37 +68,37 @@ info: 2000-01-19 03:02:01.000000000
 def time := time% 13:02:01
 
 /--
-info: 14:02:01.000000000
+info: 14:02:01:000000000
 -/
 #guard_msgs in
 #eval time + (1 : Hour.Offset)
 
 /--
-info: 12:02:01.000000000
+info: 12:02:01:000000000
 -/
 #guard_msgs in
 #eval time - (1 : Hour.Offset)
 
 /--
-info: 13:12:01.000000000
+info: 13:12:01:000000000
 -/
 #guard_msgs in
 #eval time + (10 : Minute.Offset)
 
 /--
-info: 12:52:01.000000000
+info: 12:52:01:000000000
 -/
 #guard_msgs in
 #eval time - (10 : Minute.Offset)
 
 /--
-info: 13:03:01.000000000
+info: 13:03:01:000000000
 -/
 #guard_msgs in
 #eval time + (60 : Second.Offset)
 
 /--
-info: 13:01:01.000000000
+info: 13:01:01:000000000
 -/
 #guard_msgs in
 #eval time - (60 : Second.Offset)
@@ -106,49 +106,49 @@ info: 13:01:01.000000000
 def datetimetz := date% 2000-01-20:03:02:01-03:00
 
 /--
-info: 2000-01-22 06:02:01.000000000 -0300
+info: 2000-01-22:06:02:01:000000000-03:00
 -/
 #guard_msgs in
 #eval datetimetz + (2 : Day.Offset)
 
 /--
-info: 2000-01-19 06:02:01.000000000 -0300
+info: 2000-01-19:06:02:01:000000000-03:00
 -/
 #guard_msgs in
 #eval datetimetz - (1 : Day.Offset)
 
 /--
-info: 2000-01-20 07:02:01.000000000 -0300
+info: 2000-01-20:07:02:01:000000000-03:00
 -/
 #guard_msgs in
 #eval datetimetz + (1 : Hour.Offset)
 
 /--
-info: 2000-01-20 05:02:01.000000000 -0300
+info: 2000-01-20:05:02:01:000000000-03:00
 -/
 #guard_msgs in
 #eval datetimetz - (1 : Hour.Offset)
 
 /--
-info: 2000-01-20 06:12:01.000000000 -0300
+info: 2000-01-20:06:12:01:000000000-03:00
 -/
 #guard_msgs in
 #eval datetimetz + (10 : Minute.Offset)
 
 /--
-info: 2000-01-20 05:52:01.000000000 -0300
+info: 2000-01-20:05:52:01:000000000-03:00
 -/
 #guard_msgs in
 #eval datetimetz - (10 : Minute.Offset)
 
 /--
-info: 2000-01-20 06:03:01.000000000 -0300
+info: 2000-01-20:06:03:01:000000000-03:00
 -/
 #guard_msgs in
 #eval datetimetz + (60 : Second.Offset)
 
 /--
-info: 2000-01-20 06:01:01.000000000 -0300
+info: 2000-01-20:06:01:01:000000000-03:00
 -/
 #guard_msgs in
 #eval datetimetz - (60 : Second.Offset)
