tests/lean/run/timeOperations.lean
@@ -36,97 +36,97 @@ info: 1969-12-20
 def datetime := date% 2000-01-20:03:02:01
 
 /--
-info: 2000-01-20 04:02:01.000000000
+info: 2000-01-20:04:02:01:000000000
 -/
 #guard_msgs in
 #eval datetime.addHours 1
 
 /--
-info: 2000-01-20 02:02:01.000000000
+info: 2000-01-20:02:02:01:000000000
 -/
 #guard_msgs in
 #eval datetime.subHours 1
 
 /--
-info: 2000-01-20 03:12:01.000000000
+info: 2000-01-20:03:12:01:000000000
 -/
 #guard_msgs in
 #eval datetime.addMinutes 10
 
 /--
-info: 2000-01-20 02:52:01.000000000
+info: 2000-01-20:02:52:01:000000000
 -/
 #guard_msgs in
 #eval datetime.subMinutes 10
 
 /--
-info: 2000-01-20 03:03:01.000000000
+info: 2000-01-20:03:03:01:000000000
 -/
 #guard_msgs in
 #eval datetime.addSeconds 60
 
 /--
-info: 2000-01-20 03:01:01.000000000
+info: 2000-01-20:03:01:01:000000000
 -/
 #guard_msgs in
 #eval datetime.subSeconds 60
 
 /--
-info: 2000-01-21 03:02:01.000000000
+info: 2000-01-21:03:02:01:000000000
 -/
 #guard_msgs in
 #eval datetime.addDays 1
 
 /--
-info: 2000-01-19 03:02:01.000000000
+info: 2000-01-19:03:02:01:000000000
 -/
 #guard_msgs in
 #eval datetime.subDays 1
 
 /--
-info: 2000-02-20 03:02:01.000000000
+info: 2000-02-20:03:02:01:000000000
 -/
 #guard_msgs in
 #eval datetime.addMonthsClip 1
 
 /--
-info: 1999-12-20 03:02:01.000000000
+info: 1999-12-20:03:02:01:000000000
 -/
 #guard_msgs in
 #eval datetime.subMonthsClip 1
 
 /--
-info: 2000-02-20 03:02:01.000000000
+info: 2000-02-20:03:02:01:000000000
 -/
 #guard_msgs in
 #eval datetime.addMonthsRollOver 1
 
 /--
-info: 1999-12-20 03:02:01.000000000
+info: 1999-12-20:03:02:01:000000000
 -/
 #guard_msgs in
 #eval datetime.subMonthsRollOver 1
 
 /--
-info: 2001-01-20 03:02:01.000000000
+info: 2001-01-20:03:02:01:000000000
 -/
 #guard_msgs in
 #eval datetime.addYearsClip 1
 
 /--
-info: 1999-01-20 03:02:01.000000000
+info: 1999-01-20:03:02:01:000000000
 -/
 #guard_msgs in
 #eval datetime.subYearsClip 1
 
 /--
-info: 2001-01-20 03:02:01.000000000
+info: 2001-01-20:03:02:01:000000000
 -/
 #guard_msgs in
 #eval datetime.addYearsRollOver 1
 
 /--
-info: 1999-01-20 03:02:01.000000000
+info: 1999-01-20:03:02:01:000000000
 -/
 #guard_msgs in
 #eval datetime.subYearsRollOver 1
@@ -134,134 +134,134 @@ info: 1999-01-20 03:02:01.000000000
 def time := time% 13:02:01
 
 /--
-info: 14:02:01.000000000
+info: 14:02:01:000000000
 -/
 #guard_msgs in
 #eval time.addHours 1
 
 /--
-info: 12:02:01.000000000
+info: 12:02:01:000000000
 -/
 #guard_msgs in
 #eval time.subHours 1
 
 /--
-info: 13:12:01.000000000
+info: 13:12:01:000000000
 -/
 #guard_msgs in
 #eval time.addMinutes 10
 
 /--
-info: 12:52:01.000000000
+info: 12:52:01:000000000
 -/
 #guard_msgs in
 #eval time.subMinutes 10
 
 /--
-info: 13:03:01.000000000
+info: 13:03:01:000000000
 -/
 #guard_msgs in
 #eval time.addSeconds 60
 
 /--
-info: 13:01:01.000000000
+info: 13:01:01:000000000
 -/
 #guard_msgs in
 #eval time.subSeconds 60
 
 def datetimetz := date% 2000-01-20:03:02:01-03:00
 /--
-info: 2000-01-22 06:02:01.000000000 -0300
+info: 2000-01-22:06:02:01:000000000-03:00
 -/
 #guard_msgs in
 #eval datetimetz.addDays 2
 
 /--
-info: 2000-01-19 06:02:01.000000000 -0300
+info: 2000-01-19:06:02:01:000000000-03:00
 -/
 #guard_msgs in
 #eval datetimetz.subDays 1
 
 /--
-info: 2000-02-20 06:02:01.000000000 -0300
+info: 2000-02-20:06:02:01:000000000-03:00
 -/
 #guard_msgs in
 #eval datetimetz.addMonthsClip 1
 
 /--
-info: 1999-12-20 06:02:01.000000000 -0300
+info: 1999-12-20:06:02:01:000000000-03:00
 -/
 #guard_msgs in
 #eval datetimetz.subMonthsClip 1
 
 /--
-info: 2000-02-20 06:02:01.000000000 -0300
+info: 2000-02-20:06:02:01:000000000-03:00
 -/
 #guard_msgs in
 #eval datetimetz.addMonthsRollOver 1
 
 /--
-info: 1999-12-20 06:02:01.000000000 -0300
+info: 1999-12-20:06:02:01:000000000-03:00
 -/
 #guard_msgs in
 #eval datetimetz.subMonthsRollOver 1
 
 /--
-info: 2001-01-20 06:02:01.000000000 -0300
+info: 2001-01-20:06:02:01:000000000-03:00
 -/
 #guard_msgs in
 #eval datetimetz.addYearsClip 1
 
 /--
-info: 2001-01-20 06:02:01.000000000 -0300
+info: 2001-01-20:06:02:01:000000000-03:00
 -/
 #guard_msgs in
 #eval datetimetz.addYearsClip 1
 
 /--
-info: 2001-01-20 06:02:01.000000000 -0300
+info: 2001-01-20:06:02:01:000000000-03:00
 -/
 #guard_msgs in
 #eval datetimetz.addYearsRollOver 1
 
 /--
-info: 1999-01-20 06:02:01.000000000 -0300
+info: 1999-01-20:06:02:01:000000000-03:00
 -/
 #guard_msgs in
 #eval datetimetz.subYearsRollOver 1
 
 /--
-info: 2000-01-20 07:02:01.000000000 -0300
+info: 2000-01-20:07:02:01:000000000-03:00
 -/
 #guard_msgs in
 #eval datetimetz.addHours 1
 
 /--
-info: 2000-01-20 05:02:01.000000000 -0300
+info: 2000-01-20:05:02:01:000000000-03:00
 -/
 #guard_msgs in
 #eval datetimetz.subHours 1
 
 /--
-info: 2000-01-20 06:12:01.000000000 -0300
+info: 2000-01-20:06:12:01:000000000-03:00
 -/
 #guard_msgs in
 #eval datetimetz.addMinutes 10
 
 /--
-info: 2000-01-20 05:52:01.000000000 -0300
+info: 2000-01-20:05:52:01:000000000-03:00
 -/
 #guard_msgs in
 #eval datetimetz.subMinutes 10
 
 /--
-info: 2000-01-20 06:03:01.000000000 -0300
+info: 2000-01-20:06:03:01:000000000-03:00
 -/
 #guard_msgs in
 #eval datetimetz.addSeconds 60
 
 /--
-info: 2000-01-20 06:01:01.000000000 -0300
+info: 2000-01-20:06:01:01:000000000-03:00
 -/
 #guard_msgs in
 #eval datetimetz.subSeconds 60
